\begin{eqnarray}
u^B(h^A, h^B) & = & \alpha h^B(1 - \beta h^A) - \frac{1}{2}(h^B)^2 \nonumber \\
u^B(h^A, h^B = 0 ) & = & \alpha h^B - \frac{1}{2}(h^B)^2 \nonumber \\
\mbox{FOC}: u^B_{h^B} & = & \alpha - h^B = 0 \nonumber \\
\therefore h^B &=& \alpha \nonumber \\ 
\therefore u^B(h^B = \alpha) &= & (\alpha)^2 - \frac{1}{2}(\alpha)^2 = \frac{1}{2}\alpha^2 \nonumber \\
\mbox{At } \alpha = 16 \qquad u^B_z &=& 128 \nonumber 
\end{eqnarray}


\begin{eqnarray}
u^B(h^A, h^B) & = & \alpha h^B(1 - \beta h^A) - \frac{1}{2}(h^B)^2 \nonumber \\
u^B(h^A, h^B = 0 ) & = & \alpha h^B - \frac{1}{2}(h^B)^2 \nonumber \\
\mbox{FOC}: u^B_{h^B} & = & \alpha - h^B = 0 \nonumber \\
\therefore h^B &=& \alpha \nonumber \\ 
\therefore u^B(h^B = \alpha) &= & (\alpha)^2 - \frac{1}{2}(\alpha)^2 = \frac{1}{2}\alpha^2 \nonumber \\
\mbox{At } \alpha = 16 \qquad u^B_z &=& 128 \nonumber 
\end{eqnarray}


